Hurt me plenty

src/partie5.v
@@ -6,7 +6,7 @@ Load partie4.
 Fixpoint tau_code (t: Instruction) : DeBruijn :=
     match t with
     | (Access n)=> Var n
-    | (Push cp c) => Application (tau_code cp) (tau_code c)
+    | (Push cp c) => Application (tau_code c) (tau_code cp)
     | Grab c => Lambda (tau_code c)
     end
 .
@@ -147,6 +147,12 @@ Definition correct_option_state (t: StateOption) :=
 Notation "CoSo( s )" := (correct_option_state(s)).
 
 (*
+Lemma correct_step : forall (s1: State),
+    CoS(s1) -> (exists (s2: State), step_krivine s1 = Some s2)
+.
+*)
+
+(*
 Lemma stupid_2: forall (P: Prop), forall (Q: Prop),
     P -> Q \/ P
 .
@@ -225,10 +231,10 @@ Proof.
     +   simpl. simpl in CoS_s1. intuition. unfold max_var_smaller_n in H.
         simpl in H.
         destruct H.
-        exact H0.
+        exact H.
         simpl in H.
         destruct H.
-        exact H.
+        exact H0.
 Qed.
 
 Theorem state_trans : forall (s1 s2: State),
@@ -244,12 +250,295 @@ Qed.
 
 (* 5.4 *)
 
-
-Theorem transition_beta : forall (s1 s2: State),
-    CoS(s1) -> step_krivine s1 = Some s2 -> 
-        (((tau s1) -b> (tau s2)) \/ ((tau s1) = (tau s2)))
+Lemma substitution_multiple_lambda_aux : forall (t: DeBruijn), forall (u: list DeBruijn),
+    (forall (n: nat),
+    substitution_multiple_aux (Lambda t) n u = 
+    Lambda (substitution_multiple_aux t (n + 1) u))
 .
 Proof.
+    move => t u.
+    induction u.
+    move => n.
+    simpl. reflexivity.
+    simpl. simpl in IHu.
+    move => n.
+    assert ((substitution_multiple_aux (Lambda t) (n + 1) u) = 
+        Lambda (substitution_multiple_aux t (n + 1 + 1) u)).
+    exact (IHu (n + 1)).
+    rewrite H. simpl. reflexivity.
+Qed.
+
+Lemma substitution_multiple_lambda : forall (t: DeBruijn), forall (u: list DeBruijn),
+    (forall (n: nat),
+    substitution_multiple (Lambda t) n u = 
+    Lambda (substitution_multiple t (n + 1) u))
+.
+Proof.
+    intuition.
+    unfold substitution_multiple.
+    exact (substitution_multiple_lambda_aux t u n).
+Qed.
+
+Lemma stupide : forall (t1 t2: DeBruijn), forall (u: list DeBruijn), forall (n: nat),
+    substitution_multiple_aux (Application t1 t2) n u =
+    Application (substitution_multiple_aux t1 n u)
+                (substitution_multiple_aux t2 n u)
+.
+Proof.
+    move => t1 t2 u.
+    induction u.
+    simpl. move => n. reflexivity.
+    move => n.
+    simpl.
+    rewrite (IHu (n + 1)).
+    remember (substitution
+    (Application (substitution_multiple_aux t1 (n + 1) u)
+       (substitution_multiple_aux t2 (n + 1) u)) n a) as temp.
+    unfold substitution in Heqtemp.
+    fold substitution in Heqtemp. rewrite Heqtemp. reflexivity.
+Qed.
+
+Theorem transition_beta : forall (s1: State),
+    CoS(s1) -> forall (s2: State), (step_krivine s1 = Some s2 -> 
+        (((tau s1) -b> (tau s2)) \/ ((tau s1) = (tau s2))))
+.
+Proof.
+    move => s1 CoS1 s2 eqs2.
+    destruct s1. destruct p.
+    induction i.
+    induction e.
+    case_eq n.
+    move => H.
+    simpl in eqs2. rewrite H in eqs2.
+    discriminate.
+    intuition.
+    simpl in eqs2. rewrite H in eqs2.
+    discriminate.
+
+    simpl.
+    case_eq n.
+    move => H.
+    simpl in eqs2. rewrite H in eqs2.
+    destruct p.
+    assert ((i, s0, s) = s2).
+    apply some_truc. exact eqs2.
+    rewrite <- H0. simpl. 
+    assert (tau_aux (Access 0) (Stack (i, s0) e) s = tau_aux i s0 s).
+    case_eq s.
+    intuition. unfold tau_aux.
+    simpl.
+    unfold tau_environment. unfold substitution_multiple. simpl. 
+    assert (substitution_multiple_aux (Var 0) 1 (tau_environment_aux e) = Var 0).
+    apply (substitution_multiple_C_0 (Var 0) 1). unfold max_var_smaller_n. simpl. lia.
+    simpl. intuition. lia.
+    rewrite -> H2. simpl. unfold substitution_multiple. rewrite deprotect_involutive.
+    reflexivity.
+    
+    intuition. simpl.
+    assert ((tau_environment (Stack (i, s0) e) (Var 0)) =
+        (tau_environment s0 (tau_code i))).
+    unfold tau_environment. simpl.
+    assert (substitution_multiple (Var 0) 1 (tau_environment_aux e) = Var 0).
+    apply (substitution_multiple_C_0 (Var 0) 1). unfold max_var_smaller_n. simpl. lia.
+    simpl. intuition. lia.
+    rewrite H2. simpl. rewrite deprotect_involutive. reflexivity.
+    rewrite H2. reflexivity.
+
+    right. exact H1.
+
+    intuition.
+    
+    right.
+    rewrite H in eqs2.
+    destruct p. simpl in eqs2.
+    assert ((Access n0, e, s) = s2).
+    apply (some_truc). exact eqs2.
+    rewrite <- H0. simpl. rewrite H in IHe.
+    simpl in IHe. rewrite H in CoS1. simpl in CoS1. intuition.
+    case_eq s.
+    intuition.
+    unfold tau_aux.
+    simpl. unfold tau_environment.
+    induction e.
+    intuition.
+    unfold correct_stack in H6. rewrite H7 in H5. rewrite H7 in H0.
+    simpl in H1. contradict H1.
+    assert ((~ (1 > S n0)) -> ~ C[ 1 ]( Var (S n0))).
+    apply (Decidable.contrapositive (~ (1 > S n0))).
+    unfold Decidable.decidable. lia.
+    intuition. assert (~ (1 > S n0)). lia. intuition.
+
+    destruct p.
+    case_eq e.
+    intuition.
+    admit. admit. admit.
+
+    left.
+    assert (eqs2' := eqs2).
+    simpl in eqs2.
+    case_eq s.
+    intuition.
+    rewrite H in eqs2. discriminate.
+    intuition. rewrite H in eqs2.
+    assert ((i, Stack (a, b) e, s0) = s2).
+    apply some_truc. exact eqs2.
+    rewrite <- H0. rewrite <- H0 in IHi.
+    unfold tau.
+    unfold tau_aux.
+    induction s0.
+    intuition. simpl. unfold tau_environment.
+    intuition. 
+    (*remember (tau_environment_aux (Stack (a, b) e)) as H'.*)
+    
+    rewrite (substitution_multiple_lambda (tau_code i) (tau_environment_aux e) 0).
+    simpl.
+    remember (tau_code a) [0 <-- tau_environment_aux b] as truc.
+    assert ((substitution_multiple (tau_code i) 1 (tau_environment_aux e))
+        = (tau_code i)[1 <-- (tau_environment_aux e)]).
+    admit. (* Montrer qu'on peut bien inverser une substitution multiple *)
+    rewrite H1. rewrite deprotect_involutive.
+    apply Evaluation.
+
+    intuition.
+    destruct p. intuition.
+
+    (* Marche à peu près jusque-là*)
+    admit.
+
+    (* Push *)
+
+    simpl.
+    assert (eqs2' := eqs2).
+    simpl in eqs2.
+    assert ((i2, e, Stack (i1, e) s) = s2).
+    apply some_truc. exact eqs2.
+    rewrite <- H. unfold tau.
+    simpl.
+    case_eq s.
+    intuition.
+    right.
+    unfold tau_aux.
+    remember (tau_code (Push i1 i2)) as temp.
+    unfold tau_code in Heqtemp. fold tau_code in Heqtemp.
+    rewrite Heqtemp. unfold tau_environment. 
+    remember (((Application (tau_code i2) (tau_code i1)) [0 <-- tau_environment_aux e]))
+        as temp2.
+    unfold substitution_multiple in Heqtemp2.
+    unfold substitution_multiple_aux in Heqtemp2.
+    fold substitution_multiple_aux in Heqtemp2.
+    rewrite Heqtemp2. unfold substitution_multiple.
+    rewrite stupide.
+    remember (deprotect
+    (Application
+       (substitution_multiple_aux (tau_code i2) 0 (tau_environment_aux e))
+       (substitution_multiple_aux (tau_code i1) 0 (tau_environment_aux e))) )
+       as temp3.
+    unfold deprotect in Heqtemp3.
+    fold deprotect in Heqtemp3.
+    rewrite Heqtemp3. reflexivity.
+
+    intuition.
+    left.
+    
+    
+
+    (* Fin? *)
+    unfold substitution_multiple_aux.     
+
+    
+    simpl. simpl in CoS1. intuition.
+    unfold max_var_smaller_n in H0.
+    unfold max_var_smaller_n_depth in H0. destruct H0.
+    fold max_var_smaller_n_depth in H0.
+    fold max_var_smaller_n_depth in H1.
+    simpl. intuition.
+    assert ((tau (i1, e, s)) -b> (tau s2) \/ tau (i1, e, s) = tau s2).
+    apply IHi1.
+    simpl. intuition.
+    assert ((tau (i2, e, s)) -b> (tau s2) \/ tau (i2, e, s) = tau s2).
+    apply IHi2.
+    simpl. intuition.
+
+    
+
+
+
+    rewrite substitution_multiple_C_2.
+    simpl. intuition. admit.
+    intuition. simpl.
+
+
+    assert ((substitution (substitution_multiple (Var (S n0)) 2 (tau_environment_aux s1))
+    1 (tau_code a) [0 <-- tau_environment_aux b])
+        = (substitution_multiple (Var n0) 1 (tau_environment_aux s1))).
+    
+    
+    apply aux_0.
+
+    unfold tau_environment_aux.
+    unfold substitution_multiple. simpl.
+    rewrite (substitution_multiple_C_2). 
+        simpl. intuition.
+    simpl. admit.
+    simpl.
+    case_eq e.
+    intuition.
+    rewrite H8 in H6. simpl in H6. rewrite H8 in H2.
+    
+
+    (*
+    Application (tau_environment (Stack (i, s0) e) (Var 0)) (tau_aux a b s1) =
+    Application (tau_environment s0 (tau_code i)) (tau_aux a b s1)
+    *)
+
+    assert ((tau_environment (Stack (i, s0) e) (Var 0)) =
+        (tau_environment s0 (tau_code i))).
+    unfold tau_environment.
+    simpl. assert ((substitution_multiple (Var 0) 1 (tau_environment_aux e)) = Var 0).
+    apply (substitution_multiple_C_0 (Var 0) 1). unfold max_var_smaller_n. simpl. lia.
+    simpl. intuition. lia.
+
+    rewrite H3. simpl. rewrite deprotect_involutive. reflexivity.
+
+    (*
+    Application (tau_environment (Stack (i, s0) e) (Var 0)) (tau_aux a b s1) =
+    Application (tau_environment s0 (tau_code i)) (tau_aux a b s1)
+    *)
+
+    
+
+    intuition.
+    destruct s1. destruct p.
+    induction i.
+    induction e.
+    induction s. simpl in H.
+    intuition.
+    assert (~C[0](Var n)).
+    assert (~(0 > n)). lia.
+    assert (~(0 > n) -> ~C[0](Var n)).
+    apply (Decidable.contrapositive (~C[0](Var n))). intuition. simpl.
+    intuition. exact (H4 H2).
+    contradiction.
+    
+    simpl. destruct p. simpl in H. simpl in H0.
+    case_eq n. intuition. rewrite H1 in H0. discriminate.
+    intuition. rewrite H4 in H0. discriminate.
+
+    induction s.
+    simpl. simpl in H. destruct p.
+    simpl in H0. simpl in IHe.
+    case_eq n.
+    intuition.
+    rewrite H1 in H0.
+    rewrite H1 in H5. rewrite H1 in H2.
+    apply aux_0 in H2.
+    unfold tau_environment. assert ((i, s, Nil) = s2). apply some_truc. exact H0.
+    rewrite <- H7. unfold tau. unfold tau_aux.
+
+
+
+
+
     intro s1; case s1; clear s1.
     intro p; case p; clear p.
     move => i e s.
@@ -283,7 +572,7 @@ Proof.
     intuition. simpl in H0. case_eq n.
     intuition. rewrite H1 in H0. assert ((a, b, s) = s2). admit.
     rewrite <- H2.
-    simpl. rewrite H1 in H. simpl in H.
+    simpl. rewrite H1 in H. simpl in H.some_truc
 
     induction s1. destruct a.
     induction b. 
