src/partie4.v
@@ -4,7 +4,7 @@ Load partie3.
 Fixpoint Comp (t: DeBruijn) : Instruction :=
     match t with
     | Lambda t => Grab (Comp t)
-    | Application tp1 tp2 => (Push (Comp tp1) (Comp tp2))
+    | Application tp1 tp2 => (Push (Comp tp2) (Comp tp1))
     | Var n => (Access n)
     | Protect tp => Comp tp
     end
